attempt at proving specification correctness for is_equal function

LZC.c
@@ -45,6 +45,10 @@ void encode_length(uint64_t len, uint8_t *out) {
     }
 }
 
+//  9, 101010010
+// 1001, 101010010
+// 1100001101, 101010010
+
 // bytes_to_nat
 // We need to assume that in_len <= 64 / 7 = 9.
 uint64_t decode_length(const uint8_t *in, uint64_t in_len, uint64_t *out) {
@@ -63,6 +67,14 @@ uint64_t decode_length(const uint8_t *in, uint64_t in_len, uint64_t *out) {
         }
     }
     return idx;
+}
+
+int is_equal(const uint8_t *s, const uint8_t *t, uint64_t len) {
+    if (len == 0) return 1;
+    if (s[0] != t[0]) {
+        return 0;
+    }
+    return is_equal(s + 1, t + 1, len - 1);
 }
 
 void find_largest_match(const uint8_t *in,
@@ -97,91 +109,92 @@ void find_largest_match(const uint8_t *in,
 }
 
 // compress_to_bytes
-// uint8_t *compress(const uint8_t *in, uint64_t in_len) {
-//     // TODO: Replace 65 with the correct value. 
-//     uint64_t out_len = (9 * in_len + 7) / 8 + 65;
-//     uint8_t *out = (uint8_t *)surely_malloc(out_len);
-//     uint64_t out_i = encode_length(in_len, out);
-//     uint64_t in_i = 0;
+uint8_t *compress(const uint8_t *in, uint64_t in_len) {
+    // TODO: Replace 65 with the correct value. 
+    uint64_t out_len = (9 * in_len + 7) / 8 + 65;
+    uint8_t *out = (uint8_t *)surely_malloc(out_len);
+    encode_length(in_len, out);
+    uint64_t out_i = 20;
+    uint64_t in_i = 0;
 
-//     uint8_t flag = 0;
-//     uint8_t token_count = 0;
-//     uint64_t flag_i = out_i;
-//     if (0 < in_len) out_i++;
+    uint8_t flag = 0;
+    uint8_t token_count = 0;
+    uint64_t flag_i = out_i;
+    if (0 < in_len) out_i++;
 
-//     while (in_i < in_len) {
-//         uint64_t len = 0;
-//         uint64_t off = 0;
-//         find_largest_match(in, in_len, in_i, &len, &off);
-//         if (3 <= len) {
-//             flag = flag << 1;
-//             uint64_t len_opt = len - 3;
-//             uint64_t off_opt = off - 3;
-//             out[out_i++] = (len_opt << 4) | ((uint8_t)(off_opt >> 8));
-//             out[out_i++] = (uint8_t)off_opt;
-//             in_i += len;
-//         } else {
-//             flag = (flag << 1) | 1;
-//             out[out_i++] = in[in_i++];
-//         }
+    while (in_i < in_len) {
+        uint64_t len = 0;
+        uint64_t off = 0;
+        find_largest_match(in, in_len, in_i, &len, &off);
+        if (3 <= len) {
+            flag = flag << 1;
+            uint64_t len_opt = len - 3;
+            uint64_t off_opt = off - 3;
+            out[out_i++] = (len_opt << 4) | ((uint8_t)(off_opt >> 8));
+            out[out_i++] = (uint8_t)off_opt;
+            in_i += len;
+        } else {
+            flag = (flag << 1) | 1;
+            out[out_i++] = in[in_i++];
+        }
 
-//         token_count++;
-//         if (token_count == 8) {
-//             out[flag_i] = flag;
-//             flag = 0;
-//             token_count = 0;
-//             flag_i = out_i++;
-//         }
-//     }
+        token_count++;
+        if (token_count == 8) {
+            out[flag_i] = flag;
+            flag = 0;
+            token_count = 0;
+            flag_i = out_i++;
+        }
+    }
 
-//     if (0 < token_count) {
-//         flag = flag << (8 - token_count);
-//         out[flag_i] = flag;
-//     }
+    if (0 < token_count) {
+        flag = flag << (8 - token_count);
+        out[flag_i] = flag;
+    }
 
-//     return out;
-// }
+    return out;
+}
 
-// // decompress_from_bytes
-// uint8_t *decompress(const uint8_t *in, uint64_t in_len) {
-//     uint64_t out_len = 0;
-//     uint64_t in_i = decode_length(in, in_len, &out_len);
-//     uint64_t out_i = 0;
-//     uint8_t *out = (uint8_t *)surely_malloc(out_len);
+// decompress_from_bytes
+uint8_t *decompress(const uint8_t *in, uint64_t in_len) {
+    uint64_t out_len = 0;
+    uint64_t in_i = decode_length(in, in_len, &out_len);
+    uint64_t out_i = 0;
+    uint8_t *out = (uint8_t *)surely_malloc(out_len);
 
-//     uint8_t flag = 0;
-//     uint8_t token_count = 0;
-//     uint64_t flag_i = out_i;
+    uint8_t flag = 0;
+    uint8_t token_count = 0;
+    uint64_t flag_i = out_i;
 
-//     while (out_i < out_len && in_i < in_len) {
-//         if (token_count == 0) {
-//             flag = in[in_i++];
-//             token_count = 8;
-//         }
+    while (out_i < out_len && in_i < in_len) {
+        if (token_count == 0) {
+            flag = in[in_i++];
+            token_count = 8;
+        }
 
-//         if (flag >> 7) {
-//             out[out_i++] = in[in_i++];
-//         } else {
-//             uint8_t b0 = in[in_i++];
-//             uint8_t b1 = in[in_i++];
-//             uint8_t len_opt = b0 >> 4;
-//             uint8_t off_hi = b0 & 0x0F;
-//             uint8_t off_lo = b1;
-//             uint64_t len = len_opt + 3;
-//             uint64_t off = (off_hi << 8) + off_lo + 3;
+        if (flag >> 7) {
+            out[out_i++] = in[in_i++];
+        } else {
+            uint8_t b0 = in[in_i++];
+            uint8_t b1 = in[in_i++];
+            uint8_t len_opt = b0 >> 4;
+            uint8_t off_hi = b0 & 0x0F;
+            uint8_t off_lo = b1;
+            uint64_t len = len_opt + 3;
+            uint64_t off = (off_hi << 8) + off_lo + 3;
 
-//             for (uint64_t k = 0; k < len; k++) {
-//                 out[out_i] = out[out_i - off];
-//                 out_i++;
-//             }
-//         }
+            for (uint64_t k = 0; k < len; k++) {
+                out[out_i] = out[out_i - off];
+                out_i++;
+            }
+        }
 
-//         flag <<= 1;
-//         token_count--;
-//     }
+        flag <<= 1;
+        token_count--;
+    }
 
-//     return out;
-// }
+    return out;
+}
 
 int main(void) {
 }
